theories/Example/PK/ElGamal.v
@@ -23,13 +23,13 @@ Import PackageNotation.
 #[local] Open Scope package_scope.
 Import GroupScope GRing.Theory.
 
-From NominalSSP Require Import DDH Misc Scheme.
+From NominalSSP Require Import DDH Scheme Reductions.
 
 
 Module ElGamal (GP : GroupParam).
 
 Module DDH' := DDH GP.
-Import PKScheme DDH'.
+Import PKScheme PKReductions DDH'.
 
 Module GT := GroupTheorems GP.
 Import GP GT.
@@ -62,8 +62,9 @@ Definition elgamal : pk_scheme := {|
   |}.
 
 
-Theorem correct_elgamal : CORR0 elgamal ≈₀ CORR1 elgamal.
+Theorem correct_elgamal : perfect (I_CORR elgamal) (CORR0 elgamal) (CORR1 elgamal).
 Proof.
+  eapply prove_perfect.
   apply eq_rel_perf_ind_eq.
   simplify_eq_rel m.
   apply r_const_sample_L.
@@ -78,277 +79,155 @@ Proof.
   rewrite !otf_fto expgAC -mulgA mulgV mulg1 fto_otf //.
 Qed.
 
-
-Definition stop_loc : Location := ('option 'unit; 4%N).
-
-Definition RED_loc :=
-  fset [:: stop_loc ].
+Notation init' := (
+  mpk ← get init_loc elgamal ;;
+  match mpk with
+  | None => 
+    pk ← call GETA 'unit 'el tt ;;
+    #put init_loc elgamal := Some pk ;;
+    ret pk
+  | Some pk =>
+    ret pk
+  end).
 
 Definition RED :
   module I_DDH (I_PK_OTSR elgamal) :=
-  [module RED_loc ;
+  [module fset
+    [:: flag_loc; init_loc elgamal ] ;
     #def #[ GET ] (_ : 'unit) : 'el {
-      #import {sig #[ GETA ] : 'unit → 'el } as GETA ;;
-      getNone stop_loc ;;
-      #put stop_loc := Some tt ;;
-      pk ← GETA tt ;;
+      pk ← init' ;;
       @ret 'el pk
     } ;
-    #def #[ QUERY ] (m : 'el) : 'el × 'el {
-      #import {sig #[ GETBC ] : 'unit → 'el × 'el } as GETBC ;;
-      _ ← getSome stop_loc ;;
-      '(r, sh) ← GETBC tt ;;
+    #def #[ QUERY ] (m : 'el)
+        : 'el × 'el {
+      _ ← init' ;;
+      getNone flag_loc ;;
+      #put flag_loc := Some tt ;;
+      '(r, sh) ← call
+        GETBC 'unit ('el × 'el) tt ;;
       @ret ('el × 'el) (r, op_mul m sh)
     }
   ].
 
-#[export] Instance valid_RED_DDH0
-  : ValidPackage (RED_loc :|: DDH0_loc)
-      Game_import (I_PK_OTSR elgamal) (RED ∘ DDH0)%share.
-Proof.
-  eapply valid_package_inject_locations.
-  2: nssprove_valid.
-  1: fset_solve.
-Qed.
-
-#[export] Instance valid_RED_DDH1
-  : ValidPackage (RED_loc :|: DDH1_loc)
-      Game_import (I_PK_OTSR elgamal) (RED ∘ DDH1)%share.
-Proof.
-  eapply valid_package_inject_locations.
-  2: nssprove_valid.
-  1: fset_solve.
-Qed.
-
-#[local] Hint Unfold DDH0_loc DDH1_loc PK_OTSR_loc RED_loc : in_fset_eq.
-
-Definition Rel0
-  (flag : flag_loc) (mpk : mpk_loc elgamal)
-  (stop : stop_loc) (mga : mga_loc) : Prop
-  := (isSome mpk == isSome stop)%B &&
-      if flag then stop && ~~ mga else
-        (if stop then (mpk == mga)%B else ~~ mpk).
-
 Notation inv0 := (
-  heap_ignore (PK_OTSR_loc elgamal :|: (RED_loc :|: DDH0_loc))
-  ⋊ quad flag_loc (mpk_loc elgamal) stop_loc mga_loc Rel0
+  heap_ignore (fset [:: mga_loc ])
+  ⋊ triple_rhs flag_loc (PKScheme.init_loc elgamal) mga_loc
+      (λ f pk ga, ~~ f → pk = ga)
 ).
 
-Lemma inv0_Invariant :
-  Invariant (PK_OTSR_loc elgamal) (RED_loc :|: DDH0_loc) inv0.
+Lemma PK_OTSR_RED_DDH_perfect b :
+  perfect (I_PK_OTSR elgamal) (PK_OTSR elgamal b) (RED ∘ DDH b).
 Proof.
-  ssprove_invariant; [ apply fsubsetxx | done ].
-Qed.
-
-Lemma pk_ots0_perf : PK_OTSR0 elgamal ≈₀ (RED ∘ DDH0)%share.
-Proof.
+  nssprove_share. eapply prove_perfect.
   apply (eq_rel_perf_ind _ _ inv0).
-  1: exact inv0_Invariant.
+  1: ssprove_invariant.
+  1-4: simpl.
+  1: fset_solve.
+  1: right; left; fset_solve.
+  1: left; fset_solve.
+  1: right; right; fset_solve.
+  1: done.
+
   simplify_eq_rel m.
-  1,2: ssprove_code_simpl.
-  + eapply r_get_remember_lhs => mpk.
-    eapply r_get_remember_rhs => stop.
-    eapply (rpre_learn). {
-      intros s0 s1 [[[_ I1] I2] I3].
-      rewrite /quad I2 I3 /Rel0 in I1.
-      move: I1 => /andP [I1 _].
-      apply I1.
+  - rewrite /init -lock //=.
+    apply r_get_vs_get_remember.
+    1: ssprove_invariant.
+    move=> //= pk.
+    destruct pk.
+    1: {
+      rewrite code_link_bind //=.
+      apply r_ret.
+      intros s0 s1 H.
+      split; [ done | apply H ].
     }
-    move=> /eqP ?.
-    destruct mpk, stop => //=.
-    1: apply r_fail.
-    ssprove_swap_rhs 0%N.
-    ssprove_sync => sk.
-    eapply r_put_lhs, r_put_rhs, r_put_rhs.
+    ssprove_code_simpl; simpl.
+    ssprove_sync => a.
+    apply r_put_rhs.
+    apply r_put_vs_put.
     ssprove_restore_mem.
-    2: by eapply r_ret.
+    2: by apply r_ret.
+    ssprove_invariant.
+    intros h0 h1 H f.
+    by get_heap_simpl.
 
-    ssprove_invariant. {
-      apply preserve_update_r_ignored_heap_ignore.
-      1: fset_solve.
-      apply preserve_update_r_ignored_heap_ignore.
-      1: fset_solve.
-      apply preserve_update_l_ignored_heap_ignore.
-      1: fset_solve.
-      intros h0 h1 H.
-      apply H.
-    }
-    intros s0 s1 [[I1 I2] I3].
-    rewrite /quad /Rel0 //= in I1 |- *.
-    get_heap_simpl.
-    simpl.
-    move: I1.
-    elim: (get_heap s0 flag_loc) => //= _ H.
-    rewrite /quad I2 I3 /Rel0 in H.
-    done.
-
-  + eapply r_get_remember_lhs => mpk.
-    eapply r_get_remember_rhs => stop.
-    eapply (rpre_learn). {
-      intros s0 s1 [[[_ I1] I2] I3].
-      rewrite /quad I2 I3 /Rel0 in I1.
-      move: I1 => /andP [I1 _].
-      apply I1.
-    }
-    move=> /eqP ?.
-    destruct mpk, stop => //=.
-    2: apply r_fail.
-    ssprove_code_simpl_more.
-    eapply r_get_remember_lhs => flag.
-    eapply r_get_remember_rhs => mga.
-    eapply (rpre_learn). {
-      intros h0 h1 [[[[[_ I1] I2] I3] I4] I5].
-      rewrite /quad I2 I3 I4 I5 /Rel0 in I1.
-      apply I1.
-    }
-    destruct flag, mga.
-    1,4: done.
-    1: intros _; apply r_fail.
-    move=> //= /eqP E.
-    injection E => {}E.
-    subst.
-    eapply r_put_lhs, r_put_rhs.
-    ssprove_sync => r.
-
-    ssprove_restore_mem.
-    2: by eapply r_ret.
-
-    ssprove_invariant. {
-      unfold PK_OTSR_loc, RED_loc, DDH0_loc.
-      apply preserve_update_r_ignored_heap_ignore.
-      1: fset_solve.
-      apply preserve_update_l_ignored_heap_ignore.
-      1: fset_solve.
-      intros h0 h1 H.
-      apply H.
-    }
-    intros h0 h1 [[[[I1 I2] I3] I4] I5].
-    simpl.
-    unfold quad, Rel0.
-    get_heap_simpl.
-    rewrite //= I2 I3 //.
+  - rewrite /init -lock //=.
+    apply r_get_vs_get_remember.
+    1: ssprove_invariant.
+    move=> //= pk.
+    destruct pk as [pk|].
+    1,2: ssprove_code_simpl; simpl.
+    + apply r_get_vs_get_remember.
+      1: ssprove_invariant.
+      intros f.
+      ssprove_sync => H.
+      ssprove_swap_rhs 0%N.
+      apply r_get_remember_rhs => ga.
+      eapply (r_rem_triple_rhs flag_loc (PKScheme.init_loc elgamal) mga_loc).
+      1-4: exact _.
+      move: H => /eqP H //= H'.
+      rewrite H //= in H'.
+      rewrite -H' //= => {H'} {ga}.
+      apply r_put_vs_put.
+      apply r_put_rhs.
+      ssprove_restore_mem.
+      1: {
+        ssprove_invariant.
+        intros h0 h1 [[[[[H0 H1] H2] H3] H4] H5].
+        rewrite //= /triple_rhs.
+        by get_heap_simpl.
+      }
+      destruct b; simpl.
+      * ssprove_sync => b.
+        by apply r_ret.
+      * eapply rsymmetry.
+        eapply (r_uniform_bij _ _ _ _ _ _ _ bij_op_exp) => c1.
+        eapply (r_uniform_bij _ _ _ _ _ _ _ (bij_op_mult_op_exp m)) => c2.
+        by eapply r_ret.
+    + apply r_forget_rhs, r_forget_lhs.
+      ssprove_sync => a.
+      ssprove_swap_lhs 0%N.
+      ssprove_swap_rhs 1%N.
+      ssprove_swap_rhs 0%N.
+      apply r_get_vs_get_remember.
+      1: ssprove_invariant.
+      move=> //= pk.
+      ssprove_swap_seq_rhs [:: 3%N; 2%N; 1%N ].
+      ssprove_contract_put_get_rhs.
+      ssprove_swap_lhs 0%N.
+      ssprove_swap_rhs 1%N.
+      ssprove_swap_rhs 0%N.
+      ssprove_sync => /eqP -> {pk}.
+      ssprove_code_simpl; simpl.
+      ssprove_swap_rhs 2%N.
+      ssprove_swap_rhs 1%N.
+      ssprove_contract_put_rhs.
+      apply r_put_rhs.
+      do 2 apply r_put_vs_put.
+      ssprove_restore_mem.
+      1: by ssprove_invariant.
+      destruct b; simpl.
+      * ssprove_sync => b.
+        by apply r_ret.
+      * eapply rsymmetry.
+        eapply (r_uniform_bij _ _ _ _ _ _ _ bij_op_exp) => c1.
+        eapply (r_uniform_bij _ _ _ _ _ _ _ (bij_op_mult_op_exp m)) => c2.
+        by eapply r_ret.
 Qed.
 
-Definition Rel1
-  (flag : flag_loc) (mpk : mpk_loc elgamal)
-  (stop : stop_loc) (mga : init_loc) : Prop
-  := (isSome mpk == isSome stop)%B &&
-      if flag then stop && ~~ mga else
-        (if stop then (isSome mpk == isSome mga)%B else ~~ mpk).
 
-Notation inv1 := (
-  heap_ignore (PK_OTSR_loc elgamal :|: (RED_loc :|: DDH1_loc))
-  ⋊ quad flag_loc (mpk_loc elgamal) stop_loc init_loc Rel1
-).
-
-Lemma inv1_Invariant :
-  Invariant (PK_OTSR_loc elgamal) (RED_loc :|: DDH1_loc) inv1.
-Proof.
-  ssprove_invariant; [ apply fsubsetxx | done ].
-Qed.
-
-Lemma pk_ots1_perf : PK_OTSR1 elgamal ≈₀ (RED ∘ DDH1)%share.
-Proof.
-  apply (eq_rel_perf_ind _ _ inv1).
-  1: exact inv1_Invariant.
-  simplify_eq_rel m.
-  1,2: ssprove_code_simpl.
-  + eapply r_get_remember_lhs => mpk.
-    eapply r_get_remember_rhs => stop.
-    eapply (rpre_learn). {
-      intros s0 s1 [[[_ I1] I2] I3].
-      rewrite /quad I2 I3 /Rel0 in I1.
-      move: I1 => /andP [I1 _].
-      apply I1.
-    }
-    move=> /eqP ?.
-    destruct mpk, stop => //=.
-    1: apply r_fail.
-    ssprove_swap_rhs 0%N.
-    ssprove_sync => sk.
-    eapply r_put_lhs, r_put_rhs, r_put_rhs.
-    ssprove_restore_mem.
-    2: by eapply r_ret.
-
-    ssprove_invariant. {
-      apply preserve_update_r_ignored_heap_ignore.
-      1: fset_solve.
-      apply preserve_update_r_ignored_heap_ignore.
-      1: fset_solve.
-      apply preserve_update_l_ignored_heap_ignore.
-      1: fset_solve.
-      intros h0 h1 H.
-      apply H.
-    }
-    intros s0 s1 [[I1 I2] I3].
-    rewrite /quad /Rel1 //= in I1 |- *.
-    get_heap_simpl.
-    simpl.
-    move: I1.
-    elim: (get_heap s0 flag_loc) => //= _ H.
-    rewrite /quad I2 I3 in H.
-    done.
-
-  + eapply r_get_remember_lhs => mpk.
-    eapply r_get_remember_rhs => stop.
-    eapply (rpre_learn). {
-      intros s0 s1 [[[_ I1] I2] I3].
-      rewrite /quad I2 I3 /Rel1 in I1.
-      move: I1 => /andP [I1 _].
-      apply I1.
-    }
-    move=> /eqP ?.
-    destruct mpk, stop => //=.
-    2: apply r_fail.
-    ssprove_code_simpl_more.
-    eapply r_get_remember_lhs => flag.
-    eapply r_get_remember_rhs => mga.
-    eapply (rpre_learn). {
-      intros h0 h1 [[[[[_ I1] I2] I3] I4] I5].
-      rewrite /quad I2 I3 I4 I5 /Rel1 in I1.
-      apply I1.
-    }
-    destruct flag, mga.
-    1,4: done.
-    1: intros _; apply r_fail.
-    move=> //= /eqP E.
-    eapply r_put_lhs, r_put_rhs.
-
-    ssprove_restore_mem.
-
-    2: {
-      eapply rsymmetry.
-      eapply (r_uniform_bij _ _ _ _ _ _ _ bij_op_exp) => c1.
-      eapply (r_uniform_bij _ _ _ _ _ _ _ (bij_op_mult_op_exp m)) => c2.
-      by eapply r_ret.
-    }
-
-    ssprove_invariant. {
-      unfold PK_OTSR_loc, RED_loc, DDH0_loc.
-      apply preserve_update_r_ignored_heap_ignore.
-      1: fset_solve.
-      apply preserve_update_l_ignored_heap_ignore.
-      1: fset_solve.
-      intros h0 h1 H.
-      apply H.
-    }
-    intros h0 h1 [[[[I1 I2] I3] I4] I5].
-    simpl.
-    unfold quad, Rel1.
-    get_heap_simpl.
-    rewrite //= I2 I3 //.
-Qed.
-
-Theorem elgamal_sound
-  : ∀ A : adversary (I_PK_OTSR elgamal),
+Lemma OTSR_elgamal (A : adversary (I_PK_OTSR elgamal)) :
   AdvFor (PK_OTSR elgamal) A = AdvFor DDH (A ∘ RED).
+Proof. rewrite (AdvFor_perfect PK_OTSR_RED_DDH_perfect) Adv_sep_link //. Qed.
+
+
+Theorem CPA_elgamal {n} {p} (A : adversary (I_PK_CPA elgamal)) :
+  (∀ i b, AdvFor DDH (A ∘ SLIDE elgamal i n ∘ CHOOSE elgamal b ∘ RED) <= p) →
+  AdvFor (PK_CPA elgamal n) A <= p *+ 2 *+ n.
 Proof.
-  intros A.
-  unfold AdvFor.
-  rewrite (Adv_perf_l pk_ots0_perf).
-  rewrite (Adv_perf_r pk_ots1_perf).
-  rewrite -Adv_sep_link.
-  nssprove_separate.
+  intros H.  apply Adv_CPA_OTSR_p => i b. 
+  eapply le_trans; [ apply eq_ler | apply (H i b) ].
+  rewrite /AdvFor 2!(sep_link_assoc _ _ RED).  apply (OTSR_elgamal
+    {adversary (I_PK_OTSR elgamal) ; A ∘ SLIDE elgamal i n ∘ CHOOSE elgamal b}).
 Qed.
 
 End ElGamal.
